post lemma

build.py
@@ -50,7 +50,7 @@ GEN_DIR = "gen"
 
 NL_FILES = {"arch/riscv/vale.i.dfy",
     "impl/riscv/mod32_nl_lemmas.i.dfy",
-    "impl/riscv/mod32_lemmas.i.dfy",
+    # "impl/riscv/mod32_lemmas.i.dfy",
     "lib/bv_ops_nl.dfy"}
 
 ## misc utils
